wip: Codierung über beliebige Alphabete

TM/Code/Code.v
@@ -1,261 +1,392 @@
 Require Import Prelim.
 
-(** * Suffix *)
-
-Inductive suffix (X : Type) : list X -> list X -> Type :=
-| suffix_full (xs : list X) : suffix xs xs
-| suffix_skip (xs ys : list X) (y : X) : suffix xs ys -> suffix xs (y :: ys).
-Hint Constructors suffix.
-
-Goal suffix [1;2;3] [4;5;6;1;2;3]. Proof. repeat constructor. Qed.
-
-Lemma suffix_skip' (X : Type) (x : X) (xs : list X) :
-  suffix xs (x :: xs).
-Proof. do 2 constructor. Qed.
-
-Lemma suffix_nil (X : Type) (xs : list X) : suffix [] xs.
-Proof. induction xs; auto. Qed.
-
-Lemma suffix_from_nil (X : Type) (xs : list X) : suffix xs [] -> xs = [].
-Proof. inversion 1; now subst. Qed.
-
-Lemma suffix_transitive (X : Type) (xs ys zs : list X) :
-  suffix ys xs -> suffix zs ys -> suffix zs xs.
-Proof. intros H. revert zs. induction H; auto. Qed.
-
-Lemma suffix_app (X : Type) (xs ys zs : list X) :
-  suffix xs ys -> suffix xs (zs ++ ys).
-Proof.
-  induction zs; intros H.
-  - now rewrite app_nil_l.
-  - cbn. apply suffix_skip. auto.
-Qed.
-
-Lemma list_con_neq (X : Type) (xs : list X) (x : X) :
-  xs <> x :: xs.
-Proof.
-  induction xs as [ | x' xs IH]; cbn.
-  - congruence.
-  - intros H. injection H. intros H' ->. congruence.
-Qed.
-
-Lemma list_app_neq (X : Type) (xs ys : list X) (y : X) :
-  xs <> y :: ys ++ xs.
-Proof. intros H. assert (|xs| = |y :: ys ++ xs|) as H' by congruence. cbn in *. rewrite app_length in H'. omega. Qed.
-
-Lemma suffix_length (X : Type) (xs : list X) (ys : list X) :
-  suffix xs ys -> |xs| <= |ys|.
-Proof. induction 1; cbn; omega. Qed.
-
-Lemma suffix_size_decrease (X : eqType) (xs ys : list X) :
-  xs <> ys -> suffix xs ys -> |xs| < |ys|.
-Proof.
-  intros H. induction 1.
-  - tauto.
-  - cbn. decide (xs = ys) as [->|E].
-    + omega.
-    + rewrite IHX0. omega. assumption.
-Qed.
-
-Lemma suffix_put_app (X : eqType) (xs : list X) (ys : list X) :
-  ys <> nil -> suffix (ys ++ xs) xs -> False.
-Proof.
-  intros H H'. eapply suffix_size_decrease in H'.
-  assert ((|ys|) + (|xs|) < |xs|) as H'' by now rewrite <- app_length.
-  assert (|ys| > 0). destruct ys; cbn; omega. omega.
-  destruct ys; cbn in *. tauto. intros H''. eapply list_app_neq; eauto.
-Qed.
-
-Lemma suffix_put (X : eqType) (xs : list X) (y : X) :
-  suffix (y :: xs) xs -> False.
-Proof.
-  intros H. eapply suffix_size_decrease in H. cbn in *. omega.
-  intros H'. eapply list_con_neq; eauto.
-Qed.
-
-
-(** Suffix Induction *)
-
-Inductive size_ind (X : Type) (f : X -> nat) : X -> Type :=
-| size_ind_intro (x : X) : (forall y, f y < f x -> size_ind f y) -> size_ind f x.
-
-Inductive suffix_induction (X : Type) (ys : list X) : Type :=
-| suffix_induction_con : (forall xs: list X, suffix xs ys -> xs <> ys -> suffix_induction xs) ->
-                         suffix_induction ys.
-
-(* Opaque proofes for size_Ind *)
-Lemma nat_lt_0 (n : nat) : ~n < 0. Proof. omega. Qed.
-Lemma nat_lt_tran_S (a b c : nat) : b < S c -> a < b -> a < c. Proof. omega. Qed.
-
-Lemma size_Ind (X : Type) (f : X -> nat) (x : X) : size_ind f x.
-Proof.
-  constructor.
-  generalize (f x) as n.
-  induction n; intros y B.
-  - now apply nat_lt_0 in B.
-  - constructor. intros z C. apply IHn. eapply nat_lt_tran_S; eauto.
-Defined.
-
-Lemma suffix_induction_provider (X : eqType) (ys : list X) : suffix_induction ys.
-Proof.
-  pose proof (size_Ind (@List.length X) ys) as H. induction H as [ys _ IH].
-  constructor. intros xs H1 H2. apply IH. now apply (suffix_size_decrease H2 H1).
-Defined.
-
-
 (** * Codeable Class **)
 
-Definition encoding_function (X : Type) := X -> list bool.
+Section Codeable.
 
-Definition decoding_output (X : Type) (string : list bool) :=
-  option (X * {rest : list bool & suffix rest string}).
+  Variable (sigma : finType).
+  Variable (X : Type).
 
-Definition decoding_output_proj (X : Type) :=
-  option (X * list bool).
+  Definition encoding_function := X -> list sigma.
 
-Definition decoding_function (X : Type) :=
-  forall string : list bool, decoding_output X string.
+  Class codeable :=
+    mk_codeable
+      {
+        encode : encoding_function;
+        encode_injective : forall (v1 v2 : X) (r1 r2 : list sigma), encode v1 ++ r1 = encode v2 ++ r2 -> v1 = v2 /\ r1 = r2;
+      }.
 
-Definition decoding_output_project (X : Type) (string : list bool) : decoding_output X string -> decoding_output_proj X.
-Proof. destruct 1; [ | apply None]. destruct p. apply Some. constructor. apply x. apply (projT1 s). Defined.
+  Hypothesis codeable_X : codeable.
 
-Class codeable (X : Type) :=
-  {
-    encode : encoding_function X;
-    encode_injective : forall (v1 v2 : X) (r1 r2 : list bool), encode v1 ++ r1 = encode v2 ++ r2 -> v1 = v2 /\ r1 = r2;
-  }.
-
-
-(** * Basic Encoding Functions *)
-
-Fixpoint encode_list (X : Type) (encode_entries : encoding_function X) (xs : list X) : list bool.
-Proof.
-  destruct xs.
-  - apply (false :: nil).
-  - apply (cons true). apply app. apply (encode_entries x). apply (encode_list X encode_entries xs).
-Defined.
-
-Definition encode_sum (X Y : Type) (encode_left : encoding_function X) (encode_right : encoding_function Y) (v : X + Y) : list bool.
-Proof.
-  destruct v.
-  - apply (true  :: encode_left  x).
-  - apply (false :: encode_right y).
-Defined.
-
-Definition encode_pair (X Y : Type) (encode_left : encoding_function X) (encode_right : encoding_function Y) (v : X * Y) : list bool.
-Proof. destruct v as (a,b). apply (encode_left a ++ encode_right b). Defined.
-  
-Definition encode_unit := fun _ : unit => @nil bool.
-
-
-(** * Basic Coding Instances *) 
-
-(** Lists **)
-
-Lemma encode_injective_list (X : Type) (e1 : codeable X) :
-  forall (v1 v2 : list X) (r1 r2 : list bool), encode_list encode v1 ++ r1 = encode_list encode v2 ++ r2 -> v1 = v2 /\ r1 = r2.
-Proof.
-  intros xs. induction xs as [ | x xs IH]; intros y2 r1 r2 H; cbn in *.
-  + destruct y2; cbn in *; try congruence. now inv H.
-  + destruct y2 as [ | y ys]; cbn in *; auto.
-    * congruence.
-    * inv H. rewrite <- !app_assoc in H1. apply encode_injective in H1. destruct H1 as (->&H1). apply IH in H1. intuition; congruence.
-Qed.
-
-Instance I_list (X : Type) (e1 : codeable X) : codeable (list X).
-Proof.
-  split with (encode := encode_list encode).
-  - apply encode_injective_list.
-Defined.
-
-
-(** Pair *)
-
-Lemma encode_injective_pair (X Y : Type) (e1 : codeable X) (e2 : codeable Y) :
-  forall (v1 v2 : X * Y) (r1 r2 : list bool), encode_pair encode encode v1 ++ r1 = encode_pair encode encode v2 ++ r2 -> v1 = v2 /\ r1 = r2.
-Proof.
-  intros (a1, b1) (a2, b2) r1 r2 H. unfold encode_pair in *. rewrite <- !app_assoc in H.
-  apply encode_injective in H as (->&H). apply encode_injective in H as (->&->). auto.
-Qed.
-
-Instance I_pair (X Y : Type) (e1 : codeable X) (e2 : codeable Y) : codeable (X * Y).
-Proof.
-  split with (encode := encode_pair encode encode).
-  - apply encode_injective_pair.
-Defined.
-
-
-(** Sum **)
-
-Lemma encode_injective_sum (X Y : Type) (e1 : codeable X) (e2 : codeable Y) :
-  forall (v1 v2 : X + Y) (r1 r2 : list bool), encode_sum encode encode v1 ++ r1 = encode_sum encode encode v2 ++ r2 -> v1 = v2 /\ r1 = r2.
-Proof.
-  intros [v1|v1] [v2|v2] r1 r2; unfold encode_sum; intros H1; cbn in *; inv H1; apply encode_injective in H0; intuition; congruence.
-Qed.
-
-Instance I_sum (X Y : Type) (e1 : codeable X) (e2 : codeable Y) : codeable (X + Y).
-Proof.
-  split with (encode := encode_sum encode encode).
-  - apply encode_injective_sum.
-Defined.
-
-
-(** Unit **)
-
-Lemma encode_injective_unit :
-  forall (v1 v2 : unit) (r1 r2 : list bool), encode_unit v1 ++ r1 = encode_unit v2 ++ r2 -> v1 = v2 /\ r1 = r2.
-Proof. intros () () r1 r2. auto. Qed.
-
-Instance I_unit : codeable unit.
-Proof.
-  split with (encode := encode_unit).
-  - apply encode_injective_unit.
-Defined.
-
-(** Empty Set **)
-Instance I_empty : codeable Empty_set.
-Proof.
-  split with (encode := fun x : Empty_set => match x with end).
-  - intros v1. exfalso. destruct v1.
-Defined.
-
-
-(** * Castings **)
-
-Class Cast (X Y : Type) :=
-  {
-    cast : Y -> X;
-    cast_injective : forall x1 x2, cast x1 = cast x2 -> x1 = x2;
-  }.
-
-Section I_Cast.
-  Variable (X Y : Type) (castXY : Cast X Y) (e : codeable X).
-
-  Lemma I_cast : codeable Y.
+  Lemma encode_injective' : forall v1 v2 : X, encode v1 = encode v2 -> v1 = v2.
   Proof.
-    esplit with (encode := fun y => encode (cast y)).
+    intros v1 v2 H.
+    assert (encode v1 ++ [] = encode v2 ++ []) by now rewrite !app_nil_r.
+    now apply encode_injective in H0.
+  Qed.
+
+End Codeable.
+Arguments encode { _ } { _ } { _ }.
+
+Section Encode_Fin.
+  Variable X : finType.
+
+  Lemma encode_fin_injective :
+    forall (v1 v2 : X) (r1 r2 : list X),
+      [v1] ++ r1 = [v2] ++ r2 -> v1 = v2 /\ r1 = r2.
+  Proof. firstorder; now inv H. Qed.
+
+  Instance Encode_Fin : codeable X X.
+  Proof. apply mk_codeable with (encode := fun x => [x]). apply encode_fin_injective. Defined.
+
+End Encode_Fin.
+
+
+Section RListInduction.
+  Variable X : Type.
+
+  Inductive rlist : list X -> Type :=
+  | rnil  : rlist []
+  | rcons : forall xs x, rlist xs -> rlist (xs ++ [x]).
+
+  Lemma rlist_cons (xs : list X) (x : X) :
+    rlist xs -> rlist (x :: xs).
+  Proof.
+    intros H. induction H.
+    - replace ([x]) with ([] ++ [x]). constructor. constructor. apply app_nil_l.
+    - replace (x :: xs ++ [x0]) with ((x :: xs) ++ [x0]) by reflexivity. now constructor.
+  Qed.
+
+  Lemma rlist_induction : forall xs : list X, rlist xs.
+  Proof.
+    intros xs. induction xs.
+    - constructor.
+    - now apply rlist_cons.
+  Qed.
+
+End RListInduction.
+
+
+Require Export Injection.
+
+Section Remap.
+
+  Variable (X : Type).
+  Variable (sig tau : Type).
+
+  Fixpoint remap (g : tau -> option sig) (str : list tau) : list sig * list tau :=
+    match str with
+    | nil => (nil, nil)
+    | y :: str' => match g y with
+                  | Some x => let (res1, res2) := remap g str' in (x :: res1, res2)
+                  | None => ([], str)
+                  end
+    end.
+
+  Hypothesis (inj : injection_fun sig tau).
+  Notation "'f'" := (inj_f inj). Notation "'g'" := (inj_g inj).
+
+  Lemma map_app_remap :
+    forall (str : list sig) (R : list tau),
+      let (str', r2) := remap g (map f str ++ R) in
+      { r1 : list sig | R = map f r1 ++ r2 /\ str' = str ++ r1}.
+  Proof.
+    intros str. induction str; intros; cbn in *.
+    - induction R; cbn.
+      + exists []. cbn. tauto.
+      + destruct (g a) eqn:E; cbn.
+        * destruct (remap g R). destruct IHR as (r1&->&->).
+          eexists. split; eauto. cbn. f_equal. now apply inj_inv.
+        * eexists. split; eauto. cbn. reflexivity.
+    - rewrite inj_g_adjoint.
+      specialize (IHstr R). destruct (remap g (map f str ++ R)). destruct IHstr as (r1&->&->).
+      eexists. split; eauto. 
+  Qed.
+End Remap.
+
+Section Map.
+  Variable (X : Type).
+  Variable (sig tau : finType).
+  Hypothesis (code_sig : codeable sig X).
+  Hypothesis (inj : injection_fun sig tau).
+  Notation "'f'" := (inj_f inj). Notation "'g'" := (inj_g inj).
+
+
+  Lemma encode_map_injective :
+    forall (v1 v2 : X) (r1 r2 : list tau),
+      map f (encode v1) ++ r1 = map f (encode v2) ++ r2 -> v1 = v2 /\ r1 = r2.
+  Proof.
+    intros.
+    pose proof (map_app_remap inj (encode v1) r1) as L1.
+    pose proof (map_app_remap inj (encode v2) r2) as L2.
+    destruct (remap g (map f (encode v1) ++ r1)). destruct (remap g (map f (encode v2) ++ r2)).
+    destruct L1 as (R1&L1&L1'). destruct L2 as (R2&L2&L2').
+    subst.
+  Admitted.
+    
+  Instance Encode_Map : codeable tau X.
+  Proof.
+    apply mk_codeable with (encode := fun x => map f (encode (codeable := code_sig) x)).
+    now apply encode_map_injective.
+  Defined.
+  
+End Map.
+
+
+(* TODO: Injectivity of the X coding should be enough to show that. *)
+Section Stop.
+
+  Variable X : Type.
+  Variable sig : finType.
+  (*
+  Variable enc : encoding_function sig X.
+  Hypothesis enc_injective : forall x y : X, enc x = enc y -> x = y.
+  *)
+  Hypothesis (code_X : codeable sig X).
+
+  Definition option_inj : injection_fun sig (option sig).
+  Proof.
+    apply Build_injection_fun with (inj_f := Some) (inj_g := id). firstorder.
+  Defined.
+  
+  Definition encode_stop (x : X) : list (option sig) := encode (codeable := Encode_Map code_X option_inj) x ++ [None].
+
+  Lemma encode_stop_injective :
+    forall (v1 v2 : X) (r1 r2 : list finType_CS),
+      encode_stop v1 ++ r1 = encode_stop v2 ++ r2 -> v1 = v2 /\ r1 = r2.
+  Proof.
+    intros. unfold encode_stop in H. cbn in *. rewrite <- !app_assoc in H.
+    apply (encode_injective (codeable := Encode_Map code_X option_inj)) in H as [H1 H2]. now (inv H1; inv H2).
+  Qed.
+  
+  Instance Encode_Stop : codeable (FinType (EqType (option sig))) X.
+  Proof.
+    apply mk_codeable with (encode := encode_stop). now apply encode_stop_injective.
+  Qed.
+  
+End Stop.
+
+
+
+Section Encode_Bool.
+  Lemma encode_bool_injective : forall (v1 v2 : bool) r1 r2, [v1] ++ r1 = [v2] ++ r2 -> v1 = v2 /\ r1 = r2.
+  Proof. intros v1 v2 r1 r2 H. now inv H. Qed.
+  Instance Encode_Bool : codeable (FinType (EqType bool)) bool := mk_codeable encode_bool_injective.
+End Encode_Bool.
+
+
+Section Encode_Sum.
+  Variable (X Y : Type).
+  Variable (sig tau : finType).
+  Hypothesis (code_X : codeable sig X) (code_Y : codeable tau Y).
+
+  
+  Definition encode_sum (a : X + Y) : list (sig + tau + bool) :=
+    match a with
+    | inl x => inr true  :: map (fun sig' => inl (inl sig')) (encode (codeable := code_X) x) ++ [inr  true]
+    | inr y => inr false :: map (fun tau' => inl (inr tau')) (encode (codeable := code_Y) y) ++ [inr false]
+    end.
+
+  Fixpoint undo_encode_sum_X (str : list (sig + tau + bool)) : option (list sig) * list (sig + tau + bool) :=
+    match str with
+    | nil => (None, str)
+    | inl (inl x) :: rest =>
+      match undo_encode_sum_X rest with
+      | (Some x', rest') => (Some (x :: x'), rest')
+      | (None,    rest') => (Some [x],       rest')
+      end
+    | inl (inr x) :: rest => (None, str)
+    | inr true  :: rest => (Some [], rest)
+    | inr false :: rest => (None,    str)
+    end.
+      
+  Fixpoint undo_encode_sum_Y (str : list (sig + tau + bool)) : option (list tau) * list (sig + tau + bool). Admitted.
+
+  Definition undo_encode_sum (str : list (sig + tau + bool)) : option (list (sig + tau)) * list (sig + tau + bool) :=
+    match str with
+    | inr true  :: str => match undo_encode_sum_X str with
+                         | (Some x, rest') => (Some (map inl x), rest')
+                         | (None,   rest') => (None, rest')
+                         end
+    | inr false :: str => match undo_encode_sum_Y str with
+                         | (Some y, rest') => (Some (map inr y), rest')
+                         | (None,   rest') => (None, rest')
+                         end
+    | _ => (None, str)
+    end.
+
+  (*
+  Lemma encode_sum_inv (v : X + Y) (r1 r2 : list (sig + tau + bool)) :
+    encode_sum v = r1 -> undo_encode_sum (r1 ++ r2) = (Some (map inl r1), r2).
+*)
+  
+
+  Lemma encode_sum_injective :
+    forall (v1 v2 : X + Y) (r1 r2 : list (sig + tau + bool)),
+      encode_sum v1 ++ r1 = encode_sum v2 ++ r2 -> v1 = v2 /\ r1 = r2.
+  Proof.
+    (*
+    intros [v1|v1] [v2|v2] r1 r2; intros H1; cbn in *; inv H1.
+    - 
+
+      remember (encode v1) as e1. remember (encode v2) as e2.
+      revert r1 r2 H0.
+      induction e1; intros; cbn in *.
+      + destruct e2; cbn in *.
+        * split; auto. f_equal. eapply encode_injective'. congruence.
+        * split.
+          -- f_equal. eapply encode_injective'.
+*)
+  Admitted.
+
+  Instance Encode_Sum : codeable (FinType (EqType (sig + tau + bool))) (X + Y) := mk_codeable encode_sum_injective.
+End Encode_Sum.
+
+
+Section Encode_List.
+  Variable sigma : finType.
+  Variable (X : Type) (code_X : codeable sigma X).
+
+  Fixpoint encode_list (xs : list X) : list (sigma + bool) :=
+    match xs with
+    | nil => [inr false]
+    | x :: xs' => inr true :: map inl (encode x (codeable := code_X)) ++ encode_list xs'
+    end.
+
+  Lemma encode_injective_list :
+    forall (v1 v2 : list X) (r1 r2 : list (sigma + bool)), encode_list v1 ++ r1 = encode_list v2 ++ r2 -> v1 = v2 /\ r1 = r2.
+  Proof.
+    intros xs. induction xs as [ | x xs IH]; intros y2 r1 r2 H; cbn in *.
+    + destruct y2; cbn in *; try congruence; cbn in *; try now inv H.
+    + destruct y2 as [ | y ys]; cbn in *; auto.
+      * congruence.
+      * inv H.
+        (*
+        apply encode_injective in H1.
+        rewrite <- !app_assoc in H1. apply encode_injective in H1. destruct H1 as (->&H1). apply IH in H1. intuition; congruence.
+         *)
+  Admitted.
+
+  Instance Encode_List : codeable (FinType (EqType (sigma + bool)))%type (list X) := mk_codeable encode_injective_list.
+
+End Encode_List.
+
+
+Section Encode_Pair.
+  Variable (X Y : Type) (sig : finType).
+  Hypothesis (code_X : codeable sig X) (code_Y : codeable sig Y).
+
+  Definition encode_pair (v : X * Y) : list sig.
+  Proof. destruct v as (a,b). apply (encode (codeable := code_X) a ++ encode (codeable := code_Y) b). Defined.
+
+  Lemma encode_pair_injective :
+    forall (v1 v2 : X * Y) (r1 r2 : list sig), encode_pair v1 ++ r1 = encode_pair v2 ++ r2 -> v1 = v2 /\ r1 = r2.
+  Proof.
+    intros (a1, b1) (a2, b2) r1 r2 H. unfold encode_pair in *. rewrite <- !app_assoc in H.
+    apply encode_injective in H as (->&H). apply encode_injective in H as (->&->). auto.
+  Qed.
+
+  Instance Encode_Pair : codeable sig (X * Y) := mk_codeable encode_pair_injective.
+End Encode_Pair.
+
+Section Encode_Pair'.
+  Variable (X Y : Type) (sig tau : finType).
+
+  Definition inl_inj : injection_fun sig (sig + tau).
+  Proof.
+    apply Build_injection_fun with (inj_f := inl) (inj_g := fun z => match z with inl x => Some x | _ => None end).
+    firstorder; destruct y; inv H; firstorder.
+  Defined.
+
+  Definition inr_inj : injection_fun tau (sig + tau).
+  Proof.
+    apply Build_injection_fun with (inj_f := inr) (inj_g := fun z => match z with inr x => Some x | _ => None end).
+    firstorder; destruct y; inv H; firstorder.
+  Defined.
+
+  Hypothesis (code_X : codeable sig X) (code_Y : codeable tau Y).
+
+  Instance Encode_Pair' : codeable (FinType (EqType (sig + tau)%type)) (X * Y).
+  Proof.
+    apply Encode_Pair.
+    - apply (Encode_Map _ inl_inj).
+    - apply (Encode_Map _ inr_inj).
+  Defined.
+      
+End Encode_Pair'.
+
+
+Section Encode_Unit.
+  Definition encode_unit : encoding_function (FinType (EqType Empty_set)) unit := fun _ : unit => [].
+
+  Lemma encode_unit_injective :
+    forall (v1 v2 : unit) (r1 r2 : list (FinType (EqType Empty_set))), encode_unit v1 ++ r1 = encode_unit v2 ++ r2 -> v1 = v2 /\ r1 = r2.
+  Proof. intros () () r1 r2. auto. Qed.
+
+  Instance Encode_Unit : codeable (FinType (EqType Empty_set)) unit := mk_codeable encode_unit_injective.
+
+End Encode_Unit.
+
+Section Encode_Empt.
+  Definition encode_empty : encoding_function (FinType (EqType Empty_set)) Empty_set := fun devil => match devil with end.
+
+  Lemma encode_empty_injective :
+    forall (v1 v2 : Empty_set) (r1 r2 : list (FinType (EqType Empty_set))), encode_empty v1 ++ r1 = encode_empty v2 ++ r2 -> v1 = v2 /\ r1 = r2.
+  Proof. intros v1. destruct v1. Qed.
+    
+  Instance I_empty : codeable (FinType (EqType Empty_set)) Empty_set := mk_codeable encode_empty_injective.
+End Encode_Empt.
+
+Class Cast (X Y : Type) : Type :=
+  mk_cast
+    {
+      cast_f : Y -> X;
+      cast_injective : forall x1 x2, cast_f x1 = cast_f x2 -> x1 = x2;
+    }.
+
+Instance cast_reflexive (X : Type) : Cast X X.
+Proof. hnf. apply mk_cast with (cast_f := id). firstorder. Defined.
+
+Instance cast_transitive (X Y Z : Type) : Cast X Y -> Cast Y Z -> Cast X Z.
+Proof.
+  intros C1 C2. apply mk_cast with (cast_f := fun z => cast_f (Cast := C1) (cast_f (Cast := C2) z)).
+  firstorder. now do 2 apply cast_injective.
+Defined.
+
+Section Encode_Cast.
+  Variable sig : finType.
+  Variable (X Y : Type) (castXY : Cast X Y) (e : codeable sig X).
+
+  Lemma Encode_Cast : codeable sig Y.
+  Proof.
+    esplit with (encode := fun y => encode (cast_f y)).
     - intros v1 v2 r1 r2 H. apply encode_injective in H as (H&->). split; auto. now apply cast_injective in H.
   Defined.
 
-End I_Cast.
+End Encode_Cast.
 
 Instance cast_bool : Cast (unit + unit) bool.
 Proof.
-  split with (cast := fun (b : bool) => if b then inl tt else inr tt).
+  split with (cast_f := fun (b : bool) => if b then inl tt else inr tt).
   - intros x1 x2 H. destruct x1, x2; auto; congruence.
 Defined.
 
-Instance I_bool : codeable bool.
-Proof. eapply I_cast. eapply cast_bool. auto. Defined.
+Instance I_bool : codeable (FinType (EqType bool)) bool.
+Proof. eapply Encode_Cast. shelve. eapply Encode_Bool. Unshelve. auto. Defined.
 
 Instance cast_option (X : Type) : Cast (X + unit) (option X).
 Proof.
-  split with (cast := fun p => match p with Some x => inl x | None => inr tt end).
+  split with (cast_f := fun p => match p with Some x => inl x | None => inr tt end).
   - intros [x|  ] [y| ] H; auto; congruence.
 Defined.
 
-Instance I_option (X : Type) : codeable X -> codeable (option X).
-Proof. intros H. eapply I_cast. eapply cast_option. auto. Defined.
+Instance I_option (X : Type) (sig : finType) : codeable sig X -> codeable (FinType (EqType (sig + Empty_set + bool))) (option X).
+Proof.
+  intros H. eapply Encode_Cast. eapply cast_option.
+  eapply Encode_Sum.
+  - apply H.
+  - apply Encode_Unit.
+Defined.
 
 Lemma repeat_surjective (X : Type) (x : X) (n m : nat) :
   repeat x n = repeat x m -> n = m.
@@ -267,16 +398,14 @@ Qed.
 
 Instance cast_nat : Cast (list unit) nat.
 Proof.
-  split with (cast := @List.repeat unit tt).
+  split with (cast_f := @List.repeat unit tt).
   - apply repeat_surjective.
 Defined.
 
-Instance I_nat : codeable nat.
-Proof. eapply I_cast. eapply cast_nat. auto. Defined.
+Instance I_nat : codeable (FinType (EqType (Empty_set + bool))) nat.
+Proof. eapply Encode_Cast. apply cast_nat. apply Encode_List. apply Encode_Unit. Defined.
 
-
-(* Non decodeable version *)
-Section Fin.
+Section Encode_Fin'.
   Variable (n : nat).
 
   Definition fin_to_nat : (Fin.t n) -> nat :=
@@ -292,87 +421,45 @@ Section Fin.
   
   Instance cast_Fin : Cast nat (Fin.t n).
   Proof.
-    split with (cast := fin_to_nat).
+    split with (cast_f := fin_to_nat).
     apply fin_to_nat_injective.
   Defined.
 
-  Instance I_Fin : codeable (Fin.t n).
-  Proof. eapply I_cast. eapply cast_Fin. auto. Defined.
-End Fin.
-
-(* Decodeable version *)
-Section Fin2.
-
-  Fixpoint cast_fin (n : nat) : Type :=
-    match n with
-    | 0 => Empty_set
-    | S n' => option (cast_fin n')
-    end.
-
-  Fixpoint cast_fin_codeable (n : nat) : codeable (cast_fin n) :=
-    match n with
-    | 0 => I_empty
-    | S n' => I_option (cast_fin_codeable n')
-    end.
-
-  Fixpoint fin_to_cast_fin (n : nat) (x : Fin.t n) : cast_fin n :=
-    match x with
-    | Fin.F1 => None
-    | @Fin.FS n' t => Some (@fin_to_cast_fin n' t)
-    end.
-
-  (* Compute cast_fin 2.
-  Compute fin_to_cast_fin (n := 3) (Fin.F1).
-  Compute fin_to_cast_fin (n := 3) (Fin.FS Fin.F1).
-  Compute fin_to_cast_fin (n := 3) (Fin.FS (Fin.FS Fin.F1)). *)
-
-  Fixpoint cast_fin_to_fin (n : nat) (x : cast_fin n) {struct n} : Fin.t n.
-  Proof.
-    destruct n; cbn in *; destruct x eqn:E.
-    - apply Fin.FS. apply (cast_fin_to_fin n c).
-    - apply Fin.F1.
-  Defined.
-
-  (* Compute cast_fin_to_fin (fin_to_cast_fin (n := 3) (Fin.FS Fin.F1)). *)
-
-  Lemma fin_to_cast_None (n : nat) (x : Fin.t (S n)) :
-    fin_to_cast_fin x = None -> x = Fin.F1.
-  Proof.
-    intros H. dependent induction x; auto. cbn in *. congruence.
-  Qed.
-
-  Lemma fin_to_cast_injective (n : nat) (x1 x2 : Fin.t n) :
-    fin_to_cast_fin x1 = fin_to_cast_fin x2 -> x1 = x2.
-  Proof.
-    revert x2. induction x1; intros x2 H; cbn in *.
-    - symmetry in H. eapply fin_to_cast_None in H. auto.
-    - dependent induction x2; cbn in *; auto; try congruence.
-      clear IHx2. inv H. f_equal. apply IHx1. assumption.
-  Qed.
-
-  Instance cast_fin2 (n : nat) : Cast (cast_fin n) (Fin.t n).
-  Proof.
-    split with (cast := fin_to_cast_fin (n := n)).
-    - apply fin_to_cast_injective.
-  Defined.
-
-  Instance I_Fin2 (n : nat) : codeable (Fin.t n).
-  Proof.
-    eapply I_cast. apply cast_fin2. apply cast_fin_codeable.
-  Defined.
-
-End Fin2.
+  Instance Encode_Fin' : codeable (FinType (EqType (Empty_set + bool))) (Fin.t n).
+  Proof. eapply Encode_Cast. eapply cast_Fin. auto. Defined.
+End Encode_Fin'.
 
 (** Test Playground *)
 
+Compute encode
+        (codeable := Encode_Pair (Encode_Unit) (Encode_Unit))
+        (tt, tt).
+
+Print FinType.
+Search finTypeC Fin.t.
+Search Fin.t FinType.
+
+(* TODO: How to instanciate Fin.t to finType? *)
 (*
-Compute (encode (X := list unit * (unit + unit) * (unit + unit)) ([tt;tt;tt], inr tt, inl tt)).
-
-Compute encode [true; false].
-Compute encode [inl (Some (true)); inl None; inr tt].
-
-Compute (encode (Some [inl (Some (true)); inl None; inr 42])).
-
-Compute (@encode _ (I_Fin 10) (Fin.FS (Fin.FS (Fin.FS (Fin.F1))))).
-Compute (@encode _ (I_Fin2 10) (Fin.FS (Fin.FS (Fin.FS (Fin.F1))))).
+Check Encode_Fin (FinType (Fin_finType 10)).
 *)
+Check Encode_Fin' 10.
+
+Compute
+  encode
+  (codeable := Encode_Fin 10)
+  (Fin.FS (Fin.FS (Fin.FS (Fin.F1)))).
+
+Check Encode_Pair' (Encode_List (Encode_Unit)) Encode_Unit.
+
+Compute encode
+        (codeable := Encode_Pair' (Encode_List (Encode_Unit)) Encode_Unit)
+        ([tt;tt;tt], tt).
+
+Check Encode_Bool.
+
+Compute encode true.
+
+Compute encode
+        (codeable := Encode_Pair' (Encode_List (Encode_Unit)) _)
+        ([tt;tt;tt], true).
